Isabelle2/DMultiPaxosTrace.thy
@@ -1,0 +1,398 @@
+theory DMultiPaxosTrace
+imports "~~/src/HOL/Library/FinFun_Syntax"
+begin
+
+type_synonym acc = nat
+type_synonym bal = nat
+type_synonym inst = nat
+type_synonym cmd = nat
+
+datatype msgs = 
+  Msg1a bal|
+  Msg1b acc inst bal "bal \<times> cmd option"|
+  Msg2a inst bal cmd
+
+datatype event = 
+  Propose cmd|
+  Phase1a bal|
+  Phase1b acc inst bal "bal \<times> cmd option"|
+  Phase2a inst bal cmd nat|
+  VoteCmd acc inst bal cmd
+
+(* record mp_state = 
+  ballot :: "acc \<Rightarrow> bal"
+  vote ::"acc \<Rightarrow>f inst \<Rightarrow>f bal \<Rightarrow>f cmd option"
+  network :: "msgs set"
+  propCmds :: "cmd option set"
+
+
+definition maxAcceptorVote::"acc \<Rightarrow> inst \<Rightarrow> mp_state \<Rightarrow> (bal \<times> cmd option)" where
+  "maxAcceptorVote a i s \<equiv> 
+    let bals = finfun_to_list ((vote s) $ a $ i);
+      bals_flt = (filter (\<lambda>b. (((vote s) $ a $ i) $ b) \<noteq> None) bals) @ [0];
+      maxBal = (fold max bals_flt (bals_flt!0));
+      v = (if maxBal > 0 then (((vote s) $ a $ i) $ maxBal) else None) in
+    (maxBal, v)"
+
+definition safe_at where
+  "safe_at m1bmsgs \<equiv> (let 
+    m1bnum = card m1bmsgs in
+    if (m1bnum * 2 > card accs) then True
+    else False)"
+
+definition safeVote::"msgs set \<Rightarrow> mp_state \<Rightarrow> cmd option set" where
+  "safeVote m1bmsgs state \<equiv> let 
+      m1bpair = image (\<lambda>nm. case nm of (Msg1b _ _ _ vs) \<Rightarrow> vs) m1bmsgs;
+      m1bBal = image (\<lambda>x. fst x) m1bpair;
+      maxBal = the_elem (Set.filter (\<lambda>le. \<forall>x \<in> m1bBal. x \<le> le) m1bBal);
+      maxVal = image (\<lambda>x. snd x) (Set.filter (\<lambda>le. fst le = maxBal) m1bpair);
+      safeVal = Set.remove None maxVal in
+   if (safeVal \<noteq> {}) then safeVal else propCmds state"
+
+fun transit::"event list \<Rightarrow> mp_state" where
+  "transit [] = \<lparr>ballot = (\<lambda>a. 0), vote = (K$ K$ K$ None),
+    network = {}, propCmds = {}\<rparr>"
+  |"transit (e#es) = (let s = transit es; ns = network s in
+    case e of Propose c \<Rightarrow> (let pCmds = propCmds s in
+        if Some c \<notin> pCmds then s\<lparr> propCmds := pCmds \<union> {Some c} \<rparr> else s)
+      |Phase1a b \<Rightarrow> if (b > 0 \<and> Msg1a b \<notin> ns) then s\<lparr> network := ns \<union> {Msg1a b} \<rparr> else s
+      |Phase1b a i b vs \<Rightarrow> (let (maxBal, v) = (maxAcceptorVote a i s); b' = ballot s a in 
+        if (Msg1a b \<in> ns \<and> b' < b \<and> (Msg1b a i b (maxBal, v)) \<notin> ns) 
+          then s\<lparr> ballot := (ballot s)(a := b), network := ns \<union> {Msg1b a i b (maxBal,v)} \<rparr> else s)
+      |Phase2a i b c \<Rightarrow> (let m2anum = card (Set.filter (\<lambda>nm. case nm of Msg2a i2 b2 _ \<Rightarrow> (i2 = i \<and> b2 = b)| _ \<Rightarrow> False) ns)
+        in if m2anum = 0 then (let m1bmsgs = Set.filter (\<lambda>nm. case nm of Msg1b _ i2 b2 _ \<Rightarrow> (i2 = i \<and> b2 = b)| _ \<Rightarrow> False) ns
+          in if safe_at m1bmsgs then (let safeVal = safeVote m1bmsgs s in
+            if Some c \<in> safeVal then s\<lparr> network := ns \<union> {Msg2a i b c} \<rparr> else s) else s) else s)
+      |VoteCmd a i b c \<Rightarrow> if (b = (ballot s) a \<and> Msg2a i b c \<in> ns) 
+        then s\<lparr> vote := (vote s)(a $:= ((vote s) $ a) (i $:= ((vote s) $ a $ i)(b $:= Some c))) \<rparr>
+        else s)" *)
+
+fun propCmds :: "event list \<Rightarrow> cmd option set" where
+  "propCmds [] = {}" |
+  "propCmds (e#s) = (let pCmds = propCmds s in
+    case e of Propose c \<Rightarrow> if Some c \<notin> pCmds then insert (Some c) pCmds else pCmds |  _ \<Rightarrow> pCmds)"
+
+definition safe_at where
+  "safe_at m1bmsgs nas \<equiv> (let m1bnum = card m1bmsgs in
+    if (m1bnum * 2 > nas) then True else False)"
+
+definition safeVote::"msgs set \<Rightarrow> event list \<Rightarrow> cmd option set" where
+  "safeVote m1bmsgs state \<equiv> let 
+      m1bpair = image (\<lambda>nm. case nm of (Msg1b _ _ _ vs) \<Rightarrow> vs) m1bmsgs;
+      m1bBal = image (\<lambda>x. fst x) m1bpair;
+      maxBal = the_elem (Set.filter (\<lambda>le. \<forall>x \<in> m1bBal. x \<le> le) m1bBal);
+      maxVal = image (\<lambda>x. snd x) (Set.filter (\<lambda>le. fst le = maxBal) m1bpair);
+      safeVal = Set.remove None maxVal in
+   if (safeVal \<noteq> {}) then safeVal else propCmds state"
+
+definition maxAcceptorVote::"(bal \<Rightarrow>f cmd option) \<Rightarrow> (bal \<times> cmd option)" where
+  "maxAcceptorVote vs \<equiv> 
+    let bals = finfun_to_list vs;
+      bals_flt = (filter (\<lambda>b. (vs $ b) \<noteq> None) bals) @ [0];
+      maxBal = (fold max bals_flt (bals_flt!0));
+      v = (if maxBal > 0 then (vs $ maxBal) else None) in
+    (maxBal, v)"
+
+fun ballot :: "event list \<Rightarrow> acc \<Rightarrow> bal" and
+  network :: "event list \<Rightarrow> msgs set" and
+  vote :: "event list \<Rightarrow> acc \<Rightarrow> inst \<Rightarrow> (bal \<Rightarrow>f cmd option)" where
+    "ballot [] a = 0"
+    |"ballot (e#s) a = (let b = ballot s a in
+      case e of Phase1b a' i' b' vs \<Rightarrow> if (a' = a \<and> b < b' \<and> (Msg1a b') \<in> network s) then b' else b |  _ \<Rightarrow> b)"
+    |"network [] = {}"
+    |"network (e#s) = (case e of Phase1a b \<Rightarrow> (let ns = network s in if (Msg1a b \<notin> ns) then ns \<union> {Msg1a b} else ns)
+        |Phase1b a i b vs \<Rightarrow> (let ns = network s in (if (ballot s a < b \<and> (Msg1a b) \<in> ns) then
+          (let (maxBal, v) = (maxAcceptorVote (vote s a i)) in 
+            if ((Msg1b a i b (maxBal, v)) \<notin> ns) 
+              then ns \<union> {Msg1b a i b (maxBal,v)} else ns) else ns))
+        |Phase2a i b c nas \<Rightarrow> (if card (Set.filter (\<lambda>a. case a of Msg2a i2 b2 _ \<Rightarrow> (i2 = i \<and> b2 = b)| _ \<Rightarrow> False) (network s)) = 0 then 
+          (let m1bmsgs = Set.filter (\<lambda>a. case a of Msg1b _ i2 b2 _ \<Rightarrow> (i2 = i \<and> b2 = b)| _ \<Rightarrow> False) (network s)
+            in if safe_at m1bmsgs nas then (let safeVal = safeVote m1bmsgs s in
+              if Some c \<in> safeVal then (network s) \<union> {Msg2a i b c} else (network s)) else (network s)) else (network s))
+        |_ \<Rightarrow> network s)"
+    |"vote [] a i = (K$ None)"
+    |"vote (e#s) a i = (let vs = (vote s a i) in
+        case e of VoteCmd a' i' b' c' \<Rightarrow> 
+          if (a = a' \<and> i = i' \<and> b' = (ballot s a) \<and> Msg2a i b' c' \<in> network s) then vs(b' $:= Some c') else vs
+      |_ \<Rightarrow> vs)"
+thm network.simps(2)
+lemma network_prop1[simp]:"network (Phase1a b # s) = network s \<or> network (Phase1a b # s) = network s \<union> {Msg1a b}"
+  by (smt event.simps(27) network.simps(2))
+lemma network_prop2[simp]:"network (Phase1b a i b vs # s) = network s \<or> network (Phase1b a i b vs # s) = network s \<union> {Msg1b a i b (maxAcceptorVote (vote s a i))}"
+  by (smt event.simps(28) maxAcceptorVote_def network.simps(2) split_conv)
+lemma network_prop3[simp]:"network (Phase2a i b c nas # s) = network s \<or> network (Phase2a i b c nas # s) = network s \<union> {Msg2a i b c}"
+  by (smt event.simps(29) network.simps(2))
+lemma network_prop4[simp]:"network ((Phase2a i b c nas) # es) = (if card (Set.filter (\<lambda>a. case a of Msg2a i2 b2 _ \<Rightarrow> (i2 = i \<and> b2 = b)| _ \<Rightarrow> False) (network es)) = 0 then 
+  (let m1bmsgs = Set.filter (\<lambda>a. case a of Msg1b _ i2 b2 _ \<Rightarrow> (i2 = i \<and> b2 = b)| _ \<Rightarrow> False) (network es)
+    in if safe_at m1bmsgs nas then (let safeVal = safeVote m1bmsgs es in
+      if Some c \<in> safeVal then (network es) \<union> {Msg2a i b c} else (network es)) else (network es)) else (network es))"
+using network.simps(2)[of _ es] by simp
+
+lemma vote_prop1[simp]:"vote (VoteCmd a' i' b c # s) a i = (vote s a i) \<or> vote (VoteCmd a' i' b c # s) a i = (vote s a i)(b $:= Some c)"
+  by (smt event.simps(30) vote.simps(2))
+
+lemma vote_prop2[simp]:"(vote (VoteCmd a' i' b c # s) a i) $ b = ((vote s a i) $ b) \<or> (vote (VoteCmd a' i' b c # s) a i) $ b = Some c"
+  using vote_prop1 by (metis finfun_upd_apply)
+  
+lemma set_prop[simp]:
+  assumes "m2anum = card (Set.filter (\<lambda>nm. case nm of Msg2a i2 b2 x \<Rightarrow> i2 = i \<and> b2 = b
+    | _ \<Rightarrow> False) s)" and "m2anum = 0" and "finite s"
+  shows "Msg2a i b c \<notin> s"
+proof
+  assume "Msg2a i b c \<in> s"
+  hence "Msg2a i b c \<in> (Set.filter (\<lambda>nm. case nm of Msg2a i2 b2 x \<Rightarrow> i2 = i \<and> b2 = b | _ \<Rightarrow> False) s)" by simp
+  hence "(Set.filter (\<lambda>nm. case nm of Msg2a i2 b2 x \<Rightarrow> i2 = i \<and> b2 = b | _ \<Rightarrow> False) s) \<noteq> {}" by blast
+  hence "m2anum \<noteq> 0" using assms(1,3)
+    by (simp add: Collect_mem_eq Finite_Set.card_0_eq Set.filter_def finite_Collect_conjI)
+  thus "False" using assms(2) by blast
+qed
+
+lemma set_prop1[simp]:
+  assumes "Msg2a i b c \<in> s" and "finite s"
+  shows "card (Set.filter (\<lambda>nm. case nm of Msg2a i2 b2 x \<Rightarrow> i2 = i \<and> b2 = b | _ \<Rightarrow> False) s) > 0"
+using assms set_prop by blast
+
+lemma set_prop2[simp]:
+  assumes "Set.filter (\<lambda>nm. case nm of Msg2a i2 b2 x \<Rightarrow> i2 = i \<and> b2 = b | _ \<Rightarrow> False) s \<noteq> {}" and "finite s"
+  shows "\<exists>c. Msg2a i b c \<in> s"
+using assms unfolding Set.filter_def
+proof-
+  obtain e where 1:"e \<in> {a \<in> s. case a of Msg2a i2 b2 x \<Rightarrow> i2 = i \<and> b2 = b | _ \<Rightarrow> False}" using assms(1) by fastforce
+  obtain c where "Msg2a i b c = e" using 1
+    by (smt mem_Collect_eq msgs.exhaust msgs.simps(10) msgs.simps(11) msgs.simps(12))
+  thus ?thesis using 1 mem_Collect_eq by blast
+qed
+
+lemma set_prop3[simp]:
+  assumes "card (Set.filter (\<lambda>nm. case nm of Msg2a i2 b2 x \<Rightarrow> i2 = i \<and> b2 = b | _ \<Rightarrow> False) s) > 0" and "finite s"
+  shows "\<exists>c. Msg2a i b c \<in> s"
+using set_prop2 by (metis assms(1) assms(2) card_empty less_nat_zero_code)
+
+lemma set_prop4[simp]:
+  assumes "\<forall>c. Msg2a i b c \<notin> s" and "finite s"
+  shows "card (Set.filter (\<lambda>nm. case nm of Msg2a i2 b2 x \<Rightarrow> i2 = i \<and> b2 = b | _ \<Rightarrow> False) s) = 0"
+using set_prop3 assms card_empty set_prop2 by blast
+
+lemma single_2a[simp]:
+  assumes "Msg2a i b c \<in> network s" and "finite accs" and "finite (network s)"
+  shows "card (Set.filter (\<lambda>nm. case nm of Msg2a i2 b2 _ \<Rightarrow> (i2 = i \<and> b2 = b)| _ \<Rightarrow> False) (network s)) = 1"
+using assms
+proof(induct s)
+  case Nil
+    thus ?case by (simp add: empty_iff network.simps(1))
+next
+  case (Cons e es)
+    thus ?case
+    proof(induct e arbitrary:es)
+      case Propose
+        thus ?case using event.simps(26) network.simps(2) by (metis (no_types, lifting)) 
+    next
+      case (Phase1a b')
+        have 1:"card (Set.filter (\<lambda>a. case a of Msg2a i2 b2 x \<Rightarrow> i2 = i \<and> b2 = b
+          | _ \<Rightarrow> False) (network es)) = 1" using Phase1a.prems
+            by (metis UnE finite_Un msgs.simps(7) network_prop1 singletonD)
+         have "network (Phase1a b' # es) = (network es) \<or> network (Phase1a b' # es)= network es \<union> {Msg1a b'}"
+          using network_prop1 by blast
+        thus ?case using 1 by (smt Collect_cong Set.filter_def UnCI UnE msgs.simps(10) singletonD)
+    next
+      case (Phase1b a' i' b' vs)
+        have 0:"network (Phase1b a' i' b' vs # es) = (network es) \<or> network (Phase1b a' i' b' vs # es)= network es \<union> {Msg1b a' i' b' (maxAcceptorVote (vote es a' i'))}"
+          using network_prop2 by blast
+        hence 1:"Msg2a i b c \<in> network es" using Phase1b.prems(2)
+          using UnE msgs.distinct(5) singletonD by blast
+        hence 2:"card (Set.filter (\<lambda>a. case a of Msg2a i2 b2 x \<Rightarrow> i2 = i \<and> b2 = b
+          | _ \<Rightarrow> False) (network es)) = 1" using Phase1b.prems 0 finite_Un by (metis (no_types, lifting)) 
+        thus ?case using 0 by (smt Collect_cong Set.filter_def UnCI UnE msgs.simps(11) singletonD)
+    next
+      case (VoteCmd a' i' b' c')
+        thus ?case using event.simps(30) network.simps(2) by (metis (no_types, lifting)) 
+    next
+      case (Phase2a i' b' c' nas)
+        {
+          assume "network (Phase2a i' b' c' nas # es) = network es"
+          hence "card (Set.filter (\<lambda>a. case a of Msg2a i2 b2 x \<Rightarrow> i2 = i \<and> b2 = b
+            | _ \<Rightarrow> False) (network (Phase2a i' b' c' nas # es))) = 1" using Phase2a.prems by presburger
+        }
+        moreover
+        {
+          assume 1:"network (Phase2a i' b' c' nas # es) = network es \<union> {Msg2a i' b' c'}"
+          hence 5:"card (Set.filter (\<lambda>a. case a of Msg2a i2 b2 x \<Rightarrow> i2 = i \<and> b2 = b
+            | _ \<Rightarrow> False) (network es \<union> {Msg2a i' b' c'})) = 1"
+          proof(cases "Msg2a i' b' c' \<in> network es")
+            case True
+              assume 0:"Msg2a i' b' c' \<in> network es"
+              hence "network (Phase2a i' b' c' nas # es) = network es"
+                using "1" Un_insert_right insert_absorb sup_bot_right by blast
+              thus ?thesis using 1 calculation by presburger
+          next
+            case False
+              assume 0:"Msg2a i' b' c' \<notin> network es"
+              thus ?thesis
+              proof(cases "i = i' \<and> b = b'")
+                case True
+                  assume 2:"i = i' \<and> b = b'"
+                  have 3:"card (Set.filter (\<lambda>a. case a of  Msg2a i2 b2 _ \<Rightarrow> (i2 = i \<and> b2 = b)
+                    | _ \<Rightarrow> False) (network es)) = 0"
+                  proof-
+                    {
+                      assume 3:"card (Set.filter (\<lambda>a. case a of Msg2a i2 b2 _ \<Rightarrow> (i2 = i \<and> b2 = b)
+                        | _ \<Rightarrow> False) (network es)) \<noteq> 0"
+                      hence "network ((Phase2a i b c' nas) # es) = network es" using network_prop4 by presburger
+                      hence "False" using 2 1 0 using UnI2 insertI1 by blast
+                    }
+                    thus ?thesis by blast
+                  qed
+                  have "finite (network es)" using Phase2a.prems(4) by (metis 1 finite_Un)
+                  hence "Set.filter (\<lambda>a. case a of  Msg2a i2 b2 x \<Rightarrow> i2 = i \<and> b2 = b
+                    | _ \<Rightarrow> False) (network es) = {}" using 3
+                      by (simp add: Collect_mem_eq Finite_Set.card_0_eq Set.filter_def finite_Collect_conjI)
+                  thus ?thesis using 0 1 2 Phase2a.prems(2,4)
+                    by (smt UnE card_eq_1_iff insertCI member_filter msgs.case(3) singletonD)
+              next
+                case False  
+                  assume 2:"\<not>(i = i' \<and> b = b')"
+                  hence "Msg2a i b c \<in> network es" using Phase2a.prems(2) 1 UnE msgs.inject(3) singletonD by blast
+                  hence "card (Set.filter (\<lambda>a. case a of Msg2a i2 b2 x \<Rightarrow> i2 = i \<and> b2 = b | _ \<Rightarrow> False) (network es)) = 1"
+                    using Phase2a.prems(1,3,4) by (metis "1" Un_infinite)
+                  thus ?thesis using 2 0
+                    by (smt Collect_cong Set.filter_def Un_insert_right insert_iff msgs.case(3) sup_bot.comm_neutral)
+              qed
+          qed
+        }
+        thus ?case by (metis calculation network_prop3) 
+    qed
+qed
+
+lemma single_2a_set[simp]:
+  assumes "Msg2a i b c \<in> network s" and "finite accs" and "finite (network s)"
+  shows "Set.filter (\<lambda>nm. case nm of Msg2a i2 b2 _ \<Rightarrow> (i2 = i \<and> b2 = b)| _ \<Rightarrow> False) (network s) = {Msg2a i b c}"
+proof-
+  have "card (Set.filter (\<lambda>nm. case nm of  Msg2a i2 b2 x \<Rightarrow> i2 = i \<and> b2 = b
+    | _ \<Rightarrow> False) (network s)) = 1" using assms single_2a by blast
+  thus ?thesis using assms(1,3)
+    by (smt Collect_cong Set.filter_def card_eq_1_iff mem_Collect_eq msgs.simps(12) singleton_conv2)
+qed
+
+lemma vote_msg2a[simp]:
+  assumes "((vote s) a i) $ b = Some c" and "finite accs" and "finite (network s)"
+  shows "Msg2a i b c \<in> network s"
+using assms
+proof(induct s)
+  case Nil
+    thus ?case by (simp add: finfun_const_apply option.simps(3) vote.simps(1))
+next
+  case (Cons e es)
+    thus ?case
+    proof(induct e)
+      case Propose
+        thus ?case by (metis (no_types, lifting) event.simps(26) network.simps(2) vote.simps(2))
+    next
+      case Phase1a
+        thus ?case by (metis (no_types, lifting) UnCI event.simps(27) finite_Un network_prop1 vote.simps(2))
+    next
+      case Phase1b
+        thus ?case by (metis (no_types, lifting) UnCI event.simps(28) finite_Un network_prop2 vote.simps(2))
+    next
+      case Phase2a
+        thus ?case by (smt UnCI event.simps(29) finite_Un network_prop4 vote.simps(2))
+    next
+      case VoteCmd
+        thus ?case by (smt event.simps(30) finfun_upd_apply network.simps(2) option.inject vote.simps(2))
+    qed
+qed
+  
+lemma safe_inv[simp]:
+  assumes "finite accs" and "finite (network s)" and "acc\<^sub>1 \<in> accs" and "acc\<^sub>2 \<in> accs" and "acc\<^sub>1 \<noteq> acc\<^sub>2"
+  and "cmd1 = ((vote s) acc\<^sub>1 i $ b)" and "cmd2 = ((vote s) acc\<^sub>2 i $ b)" and "cmd1 \<noteq> None" and "cmd2 \<noteq> None"
+  shows "cmd1 = cmd2"
+using assms
+proof(induct s)
+  case Nil
+    thus ?case by (simp add: vote.simps(1))
+next
+  case (Cons e es)
+    thus ?case
+    proof(induct e)
+      case Propose
+        thus ?case by (simp add: event.simps(26) network.simps(2) vote.simps(2))
+    next  
+      case Phase1a
+        thus ?case by (smt event.simps(27) finite_Un network.simps(2) vote.simps(2))
+    next
+      case Phase1b
+        have 1:"cmd1 = (vote es acc\<^sub>1 i) $ b" using Phase1b.prems(6,7) by simp
+        have "cmd2 = (vote es acc\<^sub>2 i) $ b" using Phase1b.prems(6,8) by simp
+        thus ?case using 1 Phase1b.prems by (metis finite_Un network_prop2)
+    next
+      case Phase2a
+        have 1:"cmd1 = (vote es acc\<^sub>1 i) $ b" using Phase2a.prems(6,7) by simp
+        have "cmd2 = (vote es acc\<^sub>2 i) $ b" using Phase2a.prems(7,8) by simp
+        thus ?case using 1 Phase2a.prems by (metis finite_Un network_prop3) 
+    next
+      case (VoteCmd a i' b' c)
+        thus ?case
+        proof(cases "acc\<^sub>1 = a \<and> i = i' \<and> b = b'")
+          case True
+            assume 0:"acc\<^sub>1 = a \<and> i = i' \<and> b = b'"
+            have 1:"cmd2 = (vote es acc\<^sub>2 i) $ b" using VoteCmd.prems(8,6) 0
+              by (smt event.simps(30) vote.simps(2))
+            have 2:"cmd1 = Some c \<or> cmd1 = ((vote es acc\<^sub>1 i) $ b)" using VoteCmd.prems(7) 0 vote_prop2 by blast
+            {
+              assume "cmd1 = ((vote es acc\<^sub>1 i) $ b)"
+              hence "cmd1 = cmd2" using 1 VoteCmd.prems(1,2,3,4,5,6,9,10)
+                by (simp add: event.simps(30) network.simps(2))
+            }
+            moreover
+            {
+              assume 3:"cmd1 = Some c"
+              have "Msg2a i b c \<in> network ((VoteCmd a i' b' c) # es)" using VoteCmd.prems 1 vote_msg2a 3 by blast
+              hence 4:"Msg2a i b c \<in> network es" using 1
+                by (metis (no_types, lifting) event.simps(30) network.simps(2)) 
+              have "Msg2a i b (the cmd2) \<in> network es" using 1 VoteCmd.prems(2,3,10) vote_msg2a
+                by (metis (no_types, lifting) event.simps(30) network.simps(2) option.collapse)
+              hence "Some c = cmd2" using 4assms(2,3,4,8,9) single_2a_set
+                by (metis "3" assms(6) assms(7) empty_iff insert_iff msgs.inject(3) option.collapse vote_msg2a)
+              hence "cmd1 = cmd2" using 3 by simp
+            }
+            thus ?thesis using 2 calculation by linarith
+        next
+          case False
+            assume 0:"\<not>(acc\<^sub>1 = a \<and> i = i' \<and> b = b')"
+            thus ?thesis
+            proof(cases "acc\<^sub>2 = a \<and> i = i' \<and> b = b'")
+              case True
+                assume 1:"acc\<^sub>2 = a \<and> i = i' \<and> b = b'"
+                hence 2:"i = i' \<and> b = b'" by blast
+                have 3:"cmd1 = (vote s acc\<^sub>1 i) $ b" using VoteCmd.prems(7,6) 1 assms(6) by blast
+                have 4:"cmd2 = Some c \<or> cmd2 = ((vote es acc\<^sub>2 i) $ b)" using VoteCmd.prems(8) 1 vote_prop2 by blast
+                {
+                  assume 5:"cmd2 = ((vote es acc\<^sub>2 i) $ b)"
+                  hence "cmd1 = cmd2" using VoteCmd.prems(1,2,3,4,5,6,9,10) 3
+                    by (smt True VoteCmd.prems(7) event.simps(30) network.simps(2) vote.simps(2))
+                }
+                moreover
+                {
+                  assume 5:"cmd2 = Some c"
+                  have "Msg2a i b c \<in> network ((VoteCmd a i' b' c) # es)" using VoteCmd.prems(2,3,8) 2 vote_msg2a 5 by blast
+                  hence 6:"Msg2a i b c \<in> network s" using 2 5 assms(2) assms(7) vote_msg2a by blast 
+                  have "Msg2a i b (the cmd1) \<in> network s" using 3 assms(2,3) VoteCmd.prems(2,3,9) vote_msg2a
+                    by (metis option.collapse)
+                  hence "Some c = cmd1" using 4 5 VoteCmd.prems(2,9) assms(2,3,7,8) vote_msg2a single_2a_set
+                    by (metis empty_iff insert_iff msgs.inject(3) option.collapse)
+                  hence "cmd1 = cmd2" using 5 by simp
+                }
+                thus ?thesis using 4 calculation by linarith
+            next
+              case False
+                assume 1:"\<not>(acc\<^sub>2 = a \<and> i = i' \<and> b = b')"
+                have 2:"cmd1 = (vote es acc\<^sub>1 i) $ b" using VoteCmd.prems(7) 0 vote_prop2
+                  by (smt event.simps(30) finfun_upd_apply_other vote.simps(2))
+                have "cmd2 = (vote es acc\<^sub>2 i) $ b" using VoteCmd.prems(8) 1 vote_prop2
+                  by (smt event.simps(30) finfun_upd_apply_other vote.simps(2))
+                thus ?thesis using 2 VoteCmd.prems(1,2,3,4,5,6,9,10) event.simps(30) network.simps(2) by auto
+            qed
+        qed
+    qed
+qed
+
+end
